Various cleanups

fstar/new/TreeKEM.fst
@@ -14,6 +14,7 @@ type direction = | Left | Right
 
 noeq type member_info (cs:ciphersuite) = {
   mi_public_key: hpke_public_key cs;
+  mi_version: nat;
 }
 
 //TODO: move this in Crypto.fsti?
@@ -26,9 +27,10 @@ let index_l (l:nat) = x:nat{x < pow2 l}
 
 noeq type key_package (cs:ciphersuite) (l:nat) = {
   kp_public_key: hpke_public_key cs;
-  unmerged_leafs: list (index_l l);
-  path_secret_from: direction;
-  path_secret_ciphertext: list (path_secret_ciphertext cs);
+  kp_version: nat;
+  kp_unmerged_leafs: list (index_l l);
+  kp_path_secret_from: direction;
+  kp_path_secret_ciphertext: list (path_secret_ciphertext cs);
 }
 
 noeq type tree (cs:ciphersuite) (lev:nat) =
@@ -36,8 +38,8 @@ noeq type tree (cs:ciphersuite) (lev:nat) =
   | Node: kp:option (key_package cs lev){lev>0} -> left:tree cs (lev - 1) -> right:tree cs (lev - 1) -> tree cs lev
 
 noeq type path (cs:ciphersuite) (lev:nat) =
-  | PLeaf: mi:option (member_info cs){lev=0} -> path cs lev
-  | PNode: kp:option (key_package cs lev){lev>0} -> next:path cs (lev-1) -> path cs lev
+  | PLeaf: mi:(member_info cs){lev=0} -> path cs lev
+  | PNode: kp:(key_package cs lev){lev>0} -> next:path cs (lev-1) -> path cs lev
 
 let child_index (l:pos) (i:index_l l) : index_l (l-1) & direction =
   if i < pow2 (l - 1) then (i,Left) else (i-pow2 (l-1),Right)
@@ -68,7 +70,7 @@ let rec tree_resolution #cs #l t =
   match t with
   | Leaf None -> []
   | Leaf (Some mi) -> [mi.mi_public_key]
-  | Node (Some kp) left right -> (kp.kp_public_key)::(unmerged_leafs_resolution t kp.unmerged_leafs)
+  | Node (Some kp) left right -> (kp.kp_public_key)::(unmerged_leafs_resolution t kp.kp_unmerged_leafs)
   | Node None left right -> (tree_resolution left)@(tree_resolution right)
 
 val resolution_index: #cs:ciphersuite -> #l:nat -> t:tree cs l -> index_l l -> nat_less (List.Tot.length (tree_resolution t))
@@ -77,7 +79,7 @@ let rec resolution_index #cs #l t leaf_index =
   | Leaf (Some mi) -> 0
   | Leaf None -> admit() //There should be a precondition that prevent this case
   | Node (Some kp) left right -> (
-    match find_index leaf_index kp.unmerged_leafs with
+    match find_index leaf_index kp.kp_unmerged_leafs with
     | Some res ->
       //That is currently not true because a node can contain an unmerged leaf which is actually blanked
       assume (1+res < List.Tot.length (tree_resolution t));
@@ -93,17 +95,6 @@ let rec resolution_index #cs #l t leaf_index =
       child_resolution_index
     else
       (List.Tot.length (tree_resolution left)) +child_resolution_index
-
-val apply_path: #cs:ciphersuite -> #l:nat -> index_l l -> tree cs l -> path cs l -> tree cs l
-let rec apply_path #cs #l leaf_index t p =
-  match t, p with
-  | Leaf _, PLeaf new_mi -> Leaf new_mi
-  | Node _ left right, PNode new_kp next_path ->
-    let (child_index, child_dir) = child_index l leaf_index in
-    if child_dir = Left then
-      Node new_kp (apply_path child_index left next_path) right
-    else
-      Node new_kp left (apply_path child_index right next_path)
 
 val hpke_multirecipient_encrypt_entropy_length: #cs:ciphersuite -> list (hpke_public_key cs) -> nat
 let hpke_multirecipient_encrypt_entropy_length #cs pks =
@@ -130,30 +121,31 @@ let derive_next_path_secret cs path_secret =
   res <-- derive_secret cs path_secret (string_to_bytes "path");
   return (res <: bytes)
 
-val node_encap: #cs:ciphersuite -> l:nat -> child_secret:bytes -> ad:bytes -> direction -> pks:list (hpke_public_key cs) -> randomness (hpke_multirecipient_encrypt_entropy_length pks) -> result (key_package cs l & bytes)
-let node_encap #cs l child_secret ad dir pks rand =
+val node_encap: #cs:ciphersuite -> l:nat -> version:nat -> child_secret:bytes -> ad:bytes -> direction -> pks:list (hpke_public_key cs) -> randomness (hpke_multirecipient_encrypt_entropy_length pks) -> result (key_package cs l & bytes)
+let node_encap #cs l version child_secret ad dir pks rand =
   node_secret <-- derive_next_path_secret cs child_secret;
   node_keys <-- derive_keypair_from_path_secret cs node_secret;
   ciphertext <-- hpke_multirecipient_encrypt pks bytes_empty ad node_secret rand;
   return (
     {
       kp_public_key = snd node_keys;
-      unmerged_leafs = [];
-      path_secret_from = dir;
-      path_secret_ciphertext = ciphertext;
+      kp_version = version;
+      kp_unmerged_leafs = [];
+      kp_path_secret_from = dir;
+      kp_path_secret_ciphertext = ciphertext;
     },
     node_secret
   )
 
-val node_decap: #cs:ciphersuite -> #l:nat -> child_secret:bytes -> ad:bytes -> i:nat -> dir:direction -> kp:key_package cs l{dir <> kp.path_secret_from ==> i < List.Tot.length kp.path_secret_ciphertext} -> result bytes
+val node_decap: #cs:ciphersuite -> #l:nat -> child_secret:bytes -> ad:bytes -> i:nat -> dir:direction -> kp:key_package cs l{dir <> kp.kp_path_secret_from ==> i < List.Tot.length kp.kp_path_secret_ciphertext} -> result bytes
 let node_decap #cs #l child_secret ad i dir kp =
-  if dir = kp.path_secret_from then (
+  if dir = kp.kp_path_secret_from then (
     if i <> 0 then
       fail "node_decap"
     else
       derive_next_path_secret cs child_secret
   ) else (
-    let ciphertext = List.Tot.index kp.path_secret_ciphertext i in
+    let ciphertext = List.Tot.index kp.kp_path_secret_ciphertext i in
     child_keys <-- derive_keypair_from_path_secret cs child_secret;
     let child_sk = fst child_keys in
     hpke_decrypt cs ciphertext.kem_output child_sk bytes_empty ad ciphertext.ciphertext
@@ -177,19 +169,24 @@ val update_path: #cs:ciphersuite -> #l:nat -> t:tree cs l -> leaf_index:index_l 
 let rec update_path #cs #l t leaf_index leaf_secret ad rand =
   match t with
   | Leaf None -> admit() //TODO: in the previous code, it fails in this case
-  | Leaf _ ->
+  | Leaf (Some mi) ->
     //TODO: in the previous code, it does some credential check here
     leaf_keys <-- derive_keypair_from_path_secret cs leaf_secret;
-    return (PLeaf (Some ({mi_public_key=snd leaf_keys})), leaf_secret)
-  | Node _ left right ->
+    return (PLeaf ({mi_public_key=snd leaf_keys; mi_version=mi.mi_version+1;}), leaf_secret)
+  | Node okp left right ->
+    let version =
+      match okp with
+      | None -> 0
+      | Some kp -> kp.kp_version+1
+    in
     let (next_leaf_index, dir) = child_index l leaf_index in
     let (child, sibling) = order_subtrees dir (left, right) in
     let (rand_next, rand_cur) = split_randomness rand (hpke_multirecipient_encrypt_entropy_length (tree_resolution sibling)) in
     recursive_call <-- update_path child next_leaf_index leaf_secret ad rand_next;
     let (child_path, child_path_secret) = recursive_call in
-    node_encap_call <-- node_encap l child_path_secret ad dir (tree_resolution sibling) rand_cur;
+    node_encap_call <-- node_encap l version child_path_secret ad dir (tree_resolution sibling) rand_cur;
     let (node_kp, node_path_secret) = node_encap_call in
-    return (PNode (Some node_kp) child_path, node_path_secret)
+    return (PNode node_kp child_path, node_path_secret)
 
 val root_secret: #cs:ciphersuite -> #l:nat -> t:tree cs l -> index_l l -> leaf_secret:bytes -> ad:bytes -> result (bytes)
 let rec root_secret #cs #l t leaf_index leaf_secret ad =
@@ -197,7 +194,7 @@ let rec root_secret #cs #l t leaf_index leaf_secret ad =
   | Leaf None -> fail ""
   | Leaf (Some _) -> return leaf_secret
   | Node (Some kp) left right -> begin
-    if List.Tot.mem leaf_index kp.unmerged_leafs then (
+    if List.Tot.mem leaf_index kp.kp_unmerged_leafs then (
       return leaf_secret
     ) else (
       let (next_leaf_index, dir) = child_index l leaf_index in
@@ -205,8 +202,8 @@ let rec root_secret #cs #l t leaf_index leaf_secret ad =
       child_path_secret <-- root_secret child next_leaf_index leaf_secret ad;
       //The condition is here becaus the `i` argument has not sense when dir = kp.path_secret_from.
       //Maybe we should refactor `node_decap`?
-      let i = if dir = kp.path_secret_from then 0 else resolution_index child next_leaf_index in
-      assume (List.Tot.length (tree_resolution child) == List.Tot.length kp.path_secret_ciphertext);
+      let i = if dir = kp.kp_path_secret_from then 0 else resolution_index child next_leaf_index in
+      assume (List.Tot.length (tree_resolution child) == List.Tot.length kp.kp_path_secret_ciphertext);
       node_decap child_path_secret ad i dir kp
     )
   end
